Validator/Hedge/Room.lean
@@ -1,10 +1,13 @@
+import Mathlib.Tactic.SimpRw
+
 import Validator.Std.Hedge
 
 import Validator.Regex.Room
+import Validator.Hedge.Elem
 import Validator.Hedge.Grammar
 import Validator.Hedge.IfExpr
 
-namespace Hedge.Room
+namespace Hedge.Grammar.Room
 
 def derive {α: Type}
   (G: Grammar n φ) (Φ: φ -> α -> Bool)
@@ -17,3 +20,231 @@ def derive {α: Type}
       let dchildr: Hedge.Grammar.Rule n φ := List.foldl (derive G Φ) childr children
       Hedge.Grammar.Rule.null dchildr
   ) r
+
+theorem unapply_hedge_param_and_flip
+  (G: Grammar n φ) (Φ: φ -> α -> Bool) (x: Hedge.Node α):
+  (fun (symbol: Hedge.Grammar.Symbol n φ) =>
+    match x with
+    | Hedge.Node.mk label children =>
+      let ifExpr: Hedge.Grammar.Symbol n φ := symbol
+      let childr: Hedge.Grammar.Rule n φ := Hedge.Grammar.evalif G Φ ifExpr label
+      let dchildr: Hedge.Grammar.Rule n φ := List.foldl (derive G Φ) childr children
+      Hedge.Grammar.Rule.null dchildr
+  )
+  =
+  (flip fun (symbol: Hedge.Grammar.Symbol n φ) (x': Hedge.Node α) =>
+    match x' with
+    | Hedge.Node.mk label children =>
+      let ifExpr: Hedge.Grammar.Symbol n φ := symbol
+      let childr: Hedge.Grammar.Rule n φ := Hedge.Grammar.evalif G Φ ifExpr label
+      let dchildr: Hedge.Grammar.Rule n φ := List.foldl (derive G Φ) childr children
+      Hedge.Grammar.Rule.null dchildr
+  ) x := by
+  rfl
+
+theorem derive_emptyset {α: Type} (G: Grammar n φ) (Φ: φ -> α -> Bool) (a: Hedge.Node α):
+  Hedge.Grammar.Room.derive G Φ Regex.emptyset a = Regex.emptyset := by
+  unfold derive
+  rw [unapply_hedge_param_and_flip]
+  rw [Regex.Room.derive_emptyset]
+
+theorem derive_emptystr {α: Type} (G: Grammar n φ) (Φ: φ -> α -> Bool) (a: Hedge.Node α):
+  Hedge.Grammar.Room.derive G Φ Regex.emptystr a = Regex.emptyset := by
+  unfold derive
+  rw [unapply_hedge_param_and_flip]
+  rw [Regex.Room.derive_emptystr]
+
+theorem derive_symbol {α: Type} (G: Grammar n φ) (Φ: φ -> α -> Bool) (a: Hedge.Node α):
+  Hedge.Grammar.Room.derive G Φ (Regex.symbol s) a
+    = Regex.onlyif (
+        ( match a with
+          | Node.mk label children =>
+            (List.foldl (derive G Φ) (G.evalif Φ s label) children).null
+        ) = true)
+        Regex.emptystr := by
+  unfold derive
+  rw [unapply_hedge_param_and_flip]
+  rw [Regex.Room.derive_symbol]
+
+theorem derive_or {α: Type} (G: Grammar n φ) (Φ: φ -> α -> Bool) (r1 r2: Rule n φ) (a: Hedge.Node α):
+  Hedge.Grammar.Room.derive G Φ (Regex.or r1 r2) a
+  = Regex.or (Hedge.Grammar.Room.derive G Φ r1 a) (Hedge.Grammar.Room.derive G Φ r2 a) := by
+  unfold derive
+  rw [unapply_hedge_param_and_flip]
+  rw [Regex.Room.derive_or]
+
+theorem derive_concat {α: Type} (G: Grammar n φ) (Φ: φ -> α -> Bool) (r1 r2: Rule n φ) (a: Hedge.Node α):
+  Hedge.Grammar.Room.derive G Φ (Regex.concat r1 r2) a
+    = Regex.or
+      (Regex.concat (Hedge.Grammar.Room.derive G Φ r1 a) r2)
+      (Regex.onlyif (Regex.null r1) (Hedge.Grammar.Room.derive G Φ r2 a)) := by
+  unfold derive
+  rw [unapply_hedge_param_and_flip]
+  rw [Regex.Room.derive_concat]
+
+theorem derive_star {α: Type} (G: Grammar n φ) (Φ: φ -> α -> Bool) (r1: Rule n φ) (a: Hedge.Node α):
+  Hedge.Grammar.Room.derive G Φ (Regex.star r1) a
+  = Regex.concat (Hedge.Grammar.Room.derive G Φ r1 a) (Regex.star r1) := by
+  unfold derive
+  rw [unapply_hedge_param_and_flip]
+  rw [Regex.Room.derive_star]
+
+theorem and_start {α: Type} (G: Hedge.Grammar n φ) (Φ: φ -> α -> Bool) (label: α) (children: Hedge α):
+  ((List.foldl (derive G Φ) (if Φ p label = true then G.lookup ref else Regex.emptyset) children).null = true)
+  = ((Φ p label = true) /\ ((List.foldl (derive G Φ) (G.lookup ref) children).null = true)) := by
+  generalize (Φ p label) = pred
+  generalize (G.lookup ref) = r
+  split_ifs
+  case pos h =>
+    simp_all only [true_and]
+  case neg h =>
+    simp_all only [Bool.not_eq_true, Bool.false_eq_true, false_and, eq_iff_iff, iff_false]
+    subst h
+    induction children with
+    | nil =>
+      simp only [Rule.null, List.foldl_nil, Regex.null]
+    | cons x xs ih =>
+      simp only [List.foldl_cons]
+      rw [derive_emptyset]
+      rw [ih]
+
+theorem derive_denote_symbol_is_onlyif {α: Type} (G: Hedge.Grammar n φ) (Φ: φ -> α -> Bool) (label: α) (children: Hedge α):
+  Regex.Language.derive
+    (Elem.Rule.denote G (fun s a => Φ s a = true)
+      (Regex.symbol (pred, ref))
+    )
+    (Node.mk label children)
+  =
+    Regex.Language.onlyif
+      (Φ pred label = true ∧ Elem.Rule.denote G (fun s a => Φ s a = true) (G.lookup ref) children)
+    Regex.Language.emptystr
+  := by
+  funext xs
+  rw [Hedge.Grammar.Elem.denote_symbol]
+  rw [Hedge.Language.derive_iff_tree]
+  simp only [Bool.decide_eq_true]
+
+theorem derive_commutes_symbol {α: Type}
+  (G: Hedge.Grammar n φ)
+  (Φ: φ -> α -> Bool)
+  (pred: φ)
+  (ref: Ref n)
+  (x4: Hedge.Node α)
+  (xs: Hedge α)
+  (ihr:
+    ∀ (r: Hedge.Grammar.Rule n φ) (x3: Hedge.Node.DescendantOf x4) (xs: Hedge α),
+        Hedge.Grammar.Elem.Rule.denote G (fun p a => Φ p a) (Hedge.Grammar.Room.derive G Φ r x3.val) xs
+    <-> Regex.Language.derive (Hedge.Grammar.Elem.Rule.denote G (fun p a => Φ p a) r) x3.val xs
+  )
+  :
+  Elem.Rule.denote G (fun s a => Φ s a = true) (derive G Φ (Regex.symbol (pred, ref)) x4) xs =
+  Regex.Language.derive (Elem.Rule.denote G (fun s a => Φ s a = true) (Regex.symbol (pred, ref))) x4 xs := by
+  cases x4 with
+  | mk label children =>
+
+  rw [derive_denote_symbol_is_onlyif]
+
+  rw [derive_symbol]
+  simp only
+  rw [Hedge.Grammar.Elem.denote_onlyif]
+
+  rw [Hedge.Grammar.Elem.denote_emptystr]
+  congr
+
+  simp only [evalif]
+  simp only [and_start]
+  congr
+
+  generalize G.lookup ref = r
+  induction children generalizing r with
+  | nil =>
+    simp only [List.foldl_nil]
+    rw [Hedge.Grammar.Elem.denote_nil_is_null]
+  | cons x2 xs ihxs =>
+    simp only [List.foldl]
+    rw [ihxs]
+    · have hchild := Node.Descendant.mkFirstChild_eq label x2 xs
+      have ihr := ihr (r := r) (x3 := hchild.val) (xs := xs)
+      cases hchild with
+      | mk hdes heq =>
+      rw [<- heq]
+      rw [ihr]
+      rfl
+    · intro r' x3 xs'
+      have hcons := Node.Descendant.consFirstChild_eq x2 x3
+      have ihr := ihr r' hcons.val xs'
+      cases hcons with
+      | mk hdes heq =>
+      rw [<- heq]
+      simp at ihr
+      rw [ihr]
+      rfl
+
+theorem revert_param (f g: α -> β):
+  f = g -> ∀ x, f x = g x := by
+  intro a x
+  subst a
+  simp_all only
+
+theorem derive_commutesb_iff {α: Type} (G: Hedge.Grammar n φ) (Φ: φ -> α -> Bool) (r: Hedge.Grammar.Rule n φ) (x: Hedge.Node α) (xs: Hedge α):
+  Hedge.Grammar.Elem.Rule.denote G (fun s a => Φ s a) (Hedge.Grammar.Room.derive G Φ r x) xs
+  <-> Regex.Language.derive (Hedge.Grammar.Elem.Rule.denote G (fun s a => Φ s a) r) x xs := by
+  rw [<- eq_iff_iff]
+  apply revert_param
+  induction r with
+  | emptyset =>
+    rw [derive_emptyset]
+    rw [Hedge.Grammar.Elem.denote_emptyset]
+    rw [Regex.Language.derive_emptyset]
+  | emptystr =>
+    rw [derive_emptystr]
+    rw [Hedge.Grammar.Elem.denote_emptystr]
+    rw [Hedge.Grammar.Elem.denote_emptyset]
+    rw [Regex.Language.derive_emptystr]
+  | symbol s =>
+    funext xs
+    cases s with
+    | mk pred ref =>
+    let ihr :=
+      fun (r: Hedge.Grammar.Rule n φ) (x7: Hedge.Node.DescendantOf x) (xs: Hedge α) =>
+        derive_commutesb_iff G Φ r x7 xs
+    rw [derive_commutes_symbol (ihr := ihr) (x4 := x)]
+  | or r1 r2 ih1 ih2 =>
+    rw [derive_or]
+    rw [Hedge.Grammar.Elem.denote_or]
+    rw [Hedge.Grammar.Elem.denote_or]
+    rw [Regex.Language.derive_or]
+    rw [ih1]
+    rw [ih2]
+  | concat r1 r2 ih1 ih2 =>
+    rw [derive_concat]
+    rw [Hedge.Grammar.Elem.denote_concat_n]
+    rw [Hedge.Grammar.Elem.denote_or]
+    rw [Hedge.Grammar.Elem.denote_concat_n]
+    rw [Hedge.Grammar.Elem.denote_onlyif]
+    rw [Regex.Language.derive_concat_n]
+    rw [<- ih1]
+    rw [<- ih2]
+    congr
+    apply Hedge.Grammar.Elem.null_commutes
+  | star r1 ih1 =>
+    rw [derive_star]
+    rw [Hedge.Grammar.Elem.denote_star_n]
+    rw [Hedge.Grammar.Elem.denote_concat_n]
+    rw [Hedge.Grammar.Elem.denote_star_n]
+    rw [Regex.Language.derive_star_n]
+    rw [ih1]
+  termination_by (sizeOf x, sizeOf r)
+  decreasing_by
+    apply Prod.Lex.left
+    apply Hedge.Node.DescendantOf.sizeOf
+
+theorem derive_commutesb {α: Type}
+  (G: Hedge.Grammar n φ)
+  (Φ: φ -> α -> Bool)
+  (r: Hedge.Grammar.Rule n φ)
+  (x: Hedge.Node α):
+  Hedge.Grammar.Elem.Rule.denote G (fun s a => Φ s a) (Hedge.Grammar.Room.derive G Φ r x)
+  = Regex.Language.derive (Hedge.Grammar.Elem.Rule.denote G (fun s a => Φ s a) r) x := by
+  funext xs
+  rw [derive_commutesb_iff]
